theories/MappingOneTwo.v
@@ -1,0 +1,96 @@
+From Equations Require Import Equations.
+From Prototype Require Import Prelude Sig.
+From Prototype Require LevelOne LevelTwo.
+
+Module Make (S : Sig).
+Module O := LevelOne.Make (S).
+Module T := LevelTwo.Make (S).
+
+(*********************************************************************************)
+(** *** Denotation (level two -> level one). *)
+(*********************************************************************************)
+
+Definition denote_type (k : T.kind) (s : T.scope) : Type :=
+  match k, s with 
+  | T.K_s, T.S2 n m => O.subst n m
+  | T.K_t, T.S1 n => O.term O.K_t n
+  | T.K_al tys, T.S1 n => O.term (O.K_al tys) n
+  | T.K_a ty, T.S1 n => O.term (O.K_a ty) n
+  | _, _ => False
+  end.
+  
+(** Helper lemma used to discard an impossible case in [denote]. *)
+Lemma not_K_s_S1 {n} : T.term T.K_s (T.S1 n) -> False.
+Proof. intros t ; dependent induction t ; eauto. Qed.
+    
+(** Mapping from level two terms/substitutions to level one terms/substitutions. *)
+Fixpoint denote {k s} (t : T.term k s) {struct t} : denote_type k s :=
+  match t in T.term k0 s0 return denote_type k0 s0 with
+  | T.T_var i => O.T_var i 
+  | T.T_ctor c args => O.T_ctor c (denote args)
+  | @T.T_subst _ _ T.K_t t s => O.substitute (denote t) (denote s)
+  | @T.T_subst _ _ (T.K_a ty) t s => O.substitute (denote t) (denote s)
+  | @T.T_subst _ _ (T.K_al tys) t s => O.substitute (denote t) (denote s)
+  | @T.T_subst _ _ T.K_s t s => not_K_s_S1 t
+  
+  | T.T_al_nil => O.T_al_nil
+  | T.T_al_cons a args => O.T_al_cons (denote a) (denote args)
+  
+  | T.T_abase b x => O.T_abase b x
+  | T.T_aterm t => O.T_aterm (denote t)
+  | T.T_abind a => O.T_abind (denote a)
+
+  | T.T_sshift k => O.sshift k
+  | T.T_scons t s => O.scons (denote t) (denote s)
+  | T.T_scomp s1 s2 => O.scomp (denote s1) (denote s2)
+  end.
+
+(*********************************************************************************)
+(** *** Correctness of denotation. *)
+(*********************************************************************************)
+
+(** Equality on level one terms/substitutions. We use pointwise equality 
+    for substitutions so as to not assume functional extensionality. *)
+Definition denote_rel k s : relation (denote_type k s) :=
+  match k, s with 
+  | T.K_s, T.S2 n m => @point_eq (fin n) (O.term O.K_t m)
+  | T.K_t, T.S1 n => eq
+  | T.K_a _, T.S1 n => eq 
+  | T.K_al _, T.S1 n => eq
+  | _, _ => fun _ _ => True
+  end.
+
+#[global] Instance denote_rel_equiv k s : Equivalence (denote_rel k s).
+Proof. 
+constructor ; destruct k ; destruct s ; auto.
+all: try (intros ????? ; etransitivity ; eauto).
+- intros ?. reflexivity.
+- intros ???. now symmetry.
+Qed.
+
+(** Main correctness result for [denote]: it transports level-two _sigma-equal_ terms 
+    to level-one _equal_ terms. *)
+#[global] Instance denote_proper {k s} : Proper (T.axiom_eq ==> denote_rel k s) (@denote k s).
+Proof.
+intros t1 t2 Ht. induction Ht ; simpl in * ; try auto.
+- reflexivity.
+- now symmetry.
+- etransitivity ; eauto. 
+- destruct k ; simpl ; auto.
+  + now rewrite IHHt1, IHHt2.
+  + now rewrite IHHt1, IHHt2.
+  + now rewrite IHHt1, IHHt2.
+- now rewrite IHHt1, IHHt2.
+- now rewrite IHHt1, IHHt2.
+- f_equal. apply O.substitute_proper ; auto.
+  rewrite O.up_subst_alt. reflexivity.
+- destruct k ; simpl ; solve [now setoid_rewrite O.subst_subst | auto].
+- now setoid_rewrite <-O.sshift_succ_r.
+- now setoid_rewrite O.sid_scons.
+- now setoid_rewrite O.scomp_id_l.
+- now setoid_rewrite O.scomp_id_r.
+- now setoid_rewrite O.scomp_assoc.
+- now setoid_rewrite O.scomp_scons_distrib.
+Qed.
+
+End Make.
